example fix to take into account new field in function decl

compiler_test/beepl_test/BeePL_add_ptr.v
@@ -50,7 +50,8 @@ Definition f_add : BeePL.function := {|
                                                 (Prim (Bop Cop.Oadd) 
                                                       (Var _x tint32s :: 
                                                        Var _y tint32s :: nil) tint32s)
-                                                (Var _r tint32s) tint32s |}.
+                                                (Var _r tint32s) tint32s;
+                                   is_ebpf := false |}.
 
 Definition f_main : BeePL.function := {| 
                                    fn_return := tint32s;
@@ -70,7 +71,8 @@ Definition f_main : BeePL.function := {|
                                                          (App (Var _fp (tpfun (tint32s :: tint32s :: nil) nil tint32s))
                                                             (Var _a tint32s :: 
                                                             Var _a tint32s :: nil) tint32s)
-                                                         (Var _r tint32s) tint32s) tint32s) tint32s |}.
+                                                         (Var _r tint32s) tint32s) tint32s) tint32s;
+                                  is_ebpf := false |}.
 
 Definition global_definitions : list (ident * AST.globdef BeePL.fundef type) 
    := (_add, AST.Gfun(BeePL.Internal (f_add))) ::
@@ -87,7 +89,7 @@ Proof.
   unfold build_bcomposite_env; simpl; reflexivity.
 Qed.
 
-Definition example1 : BeePL.program := @mkbprogram bcomposites 
+(*Definition example1 : BeePL.program := @mkbprogram bcomposites 
                                                    global_definitions 
                                                    public_idents 
                                                    _main 
@@ -95,4 +97,4 @@ Definition example1 : BeePL.program := @mkbprogram bcomposites
                                                    ident_to_string.
 
 
-(*Compute (type_check_program example1).*) (* Type checks *)
+Compute (type_check_program example1).*)  (* Type checks! *)
