compiler_test/beepl_test/BeePL_progs.v
@@ -2,12 +2,10 @@ Require Import AST Maps Ctypes.
 Require Import BeePL BeeTypes Errors BeePL_typechecker Csyntaxdefs. 
 From Coq Require Import String.
 
-(*Require Import BeePL_add BeePL_add_ptr BeePL_div_zero1 BeePL_div_zero BeePL_add_ex1
+Require Import BeePL_add BeePL_add_ptr BeePL_div_zero1 BeePL_div_zero BeePL_add_ex1
 BeePL_cond BeePL_app BeePL_funptr_ex1 BeePL_bpf_get_prandom BeePL_for_ex1 BeePL_for_ex2
 BeePL_external_call BeePL_match_fail_ex1 BeePL_null_ptr BeePL_bitstring1 BeePL_globvar1
-BeePL_globvar2. *)
-
-Require Import BeePL_bitstring1.
+BeePL_globvar2. 
 
 
 
@@ -32,11 +30,11 @@ Require Import BeePL_bpf_get_prandom BeePL_bpf_ktime_get_ns.*) (*BeePL_null_ptr 
 
 (* Construct the BeePL.program *)
 
-Definition example1 : BeePL.program := @mkbprogram BeePL_bitstring1.bcomposites 
-                                                   BeePL_bitstring1.global_definitions 
-                                                   BeePL_bitstring1.public_idents 
-                                                   BeePL_bitstring1._main 
-                                                   BeePL_bitstring1.bcomposite_correct
-                                                   BeePL_bitstring1.ident_to_string.
+Definition example1 : BeePL.program := @mkbprogram BeePL_div_zero.bcomposites 
+                                                   BeePL_div_zero.global_definitions 
+                                                   BeePL_div_zero.public_idents 
+                                                   BeePL_div_zero._main 
+                                                   BeePL_div_zero.bcomposite_correct
+                                                   BeePL_div_zero.ident_to_string.
 
 
