compiler_test/beepl_test/BeePL_bitstring1.v
@@ -37,11 +37,10 @@ Definition f_bytes : BeePL.function := {| fn_return := tint32s;
                                            fn_callconv := cc_default;
                                            fn_args := (_ctx, tpstruct _xdp_md_bee)  :: nil ;
                                            fn_vars := (_cv, Stype _dstruct noattr) :: (_data, Bytes) :: nil;  
-                                           fn_body := (*Bind _cv (Stype _dstruct noattr)*)
+                                           fn_body := 
                                                         (Match (Sfield (Var _ctx (tpstruct _xdp_md_bee)) _data Bytes)  
                                                          (Pbytes _cv (Stype _dstruct noattr) ((_dst, tint32s) :: (_src, tint32s) :: nil) :: nil)  
                                                          (cint (Int.repr 1) tint32s :: cint (Int.repr 2) tint32s :: nil) tint32s);
-                                                        (*(Var _cv (Stype _dstruct noattr)) (Stype _dstruct noattr)*)
                                            is_ebpf := true; 
                                                        |}.
                                                       
